engine/PrisonersDilemma/Models/Bots/DefectBot.lean
@@ -1,17 +1,17 @@
 import PrisonersDilemma.StrategyDSL
 
-namespace PD.Models.CooperateBot
+namespace PD.Models.Bots.DefectBot
 
 open PD
 open PD.Action
 open PD.StrategyDSL
 
-@[simp] def strategy : ActionExpr := ActionExpr.actionLit C
+@[simp] def strategy : ActionExpr := ActionExpr.actionLit D
 
 @[simp] def source : SourceAST :=
-  { tag := SourceTag.cooperateTag, strategy := strategy }
+  { tag := SourceTag.defectTag, strategy := strategy }
 
 @[simp] def action (oppSource : SourceAST) : Action :=
   actionFor strategy oppSource
 
-end PD.Models.CooperateBot
+end PD.Models.Bots.DefectBot
